![[Pasted image 20260119172134.png]]
Here is the comprehensive explanation of the examples and exercises found in Chapter 7 (Magnetostatic Fields) based on the provided images.

---

### **Overview: Biot-Savart Law and Magnetic Field Intensity**

These examples utilize the Biot-Savart Law and the superposition principle to calculate the Magnetic Field Intensity ($\mathbf{H}$) generated by current-carrying conductors.

**Key Formulas used:**
1.  **Infinite Line Current:** $$ \mathbf{H} = \frac{I}{2\pi\rho} \mathbf{a}_\phi $$
2.  **Semi-Infinite Line Current (endpoint at origin):** $$ \mathbf{H} = \frac{I}{4\pi\rho} \mathbf{a}_\phi $$
3.  **Finite Line Segment:** $$ \mathbf{H} = \frac{I}{4\pi\rho} (\cos\alpha_2 - \cos\alpha_1) \mathbf{a}_\phi $$
4.  **Circular Loop (on axis):** $$ \mathbf{H} = \frac{I \rho^2}{2(\rho^2 + h^2)^{3/2}} \mathbf{a}_z $$

---

### **Example 7.2: Find $\mathbf{H}$ at $(-3, 4, 0)$ due to the current filament shown in Figure 7.7(a).**

*Context:* A current filament carries a current $I = 3 \text{ A}$. The current flows along the positive $x$-axis toward the origin, and then up the positive $z$-axis away from the origin.   
![[Pasted image 20260119193638.png]]
We apply the principle of **superposition**. The total magnetic field is the sum of the fields contributed by the two distinct sections of the wire:
$$ \mathbf{H} = \mathbf{H}_1 + \mathbf{H}_2 $$
Where:
*   $\mathbf{H}_1$ is the field due to the semi-infinite wire on the $x$-axis.
*   $\mathbf{H}_2$ is the field due to the semi-infinite wire on the $z$-axis.

#### **1. Analysis of $\mathbf{H}_2$ (The $z$-axis segment)**
This segment is a semi-infinite line end at the origin ($z=0$) and from $\infty$.

*   **Observation Point ($P$):** $(-3, 4, 0)$.
*   **Radial Distance ($\rho$):** The distance from the $z$-axis to $P$.
    $$ \rho = \sqrt{(-3)^2 + 4^2} = \sqrt{9 + 16} = \sqrt{25} = 5 $$
*   **Angles:** Since the wire starts at the origin and goes to infinity:
    *   $\alpha_1 = 90^\circ$ (at the origin, relative to the vector to P).
    *   $\alpha_2 = 0^\circ$ (at infinity).
    *   Using the formula: $\mathbf{H} = \frac{I}{4\pi\rho} (\cos\alpha_2 - \cos\alpha_1)a_\phi$? The book simplifies this for a semi-infinite wire starting at the origin as just $\frac{I}{4\pi\rho}a_\phi$.
    *   Magnitude: $$ H_2 = \frac{3}{4\pi(5)} (1 - 0) = \frac{3}{20\pi} \text{ A/m} $$
*   **Direction ($\mathbf{a}_{\phi}$):**
    Using the cross product rule $\mathbf{a}_{\phi} = \mathbf{a}_l \times \mathbf{a}_\rho$.
    *   Current direction $\mathbf{a}_l = \mathbf{a}_z$.
    *   Radial vector from axis to point: $\mathbf{r} = -3\mathbf{a}_x + 4\mathbf{a}_y$.
    *   Unit radial vector $\mathbf{a}_\rho = \frac{-3\mathbf{a}_x + 4\mathbf{a}_y}{5}$.
    $$ \mathbf{a}_{\phi} = -\mathbf{a}_z \times \left( -\frac{3}{5}\mathbf{a}_x + \frac{4}{5}\mathbf{a}_y \right) = \frac{3}{5}(\mathbf{a}_z \times \mathbf{a}_x) - \frac{4}{5}(\mathbf{a}_z \times \mathbf{a}_y) $$
    $$ \mathbf{a}_{\phi} = \frac{3}{5}(\mathbf{a}_y) - \frac{4}{5}(-\mathbf{a}_x) = \frac{4}{5}\mathbf{a}_x +\frac{3}{5}\mathbf{a}_y $$
*   **Calculating $\mathbf{H}_2$:**
    $$ \mathbf{H}_2 = \frac{3}{20\pi} \left( \frac{4}{5}\mathbf{a}_x + \frac{3}{5}\mathbf{a}_y \right) $$
    $$ \mathbf{H}_2 = 38.2\mathbf{a}_x + 28.65\mathbf{a}_y \text{ mA/m} $$
 

#### **2. Analysis of $\mathbf{H}_1$ (The $x$-axis segment)**
This segment lies on the positive $x$-axis. The point $P(-3, 4, 0)$ is **not** at the "end" of this semi-infinite wire (which ends at $x=0$). The point has an $x$-coordinate of $-3$, meaning it is "behind" the termination point.

*   **Geometry:**
    *   Current flows along the $x$-axis from the origin.
    *   Distance from wire (which is on $x$-axis) to point $P(-3, 4, 0)$ is simply the distance in $y$ and $z$. Since $z=0$, distance is $y=4$. So $\rho = 4$.
*   **Angles:**
    *   Wire extends to $x = +\infty$ from $x = 0$. Point is at $x = -3$.
    *   $\alpha_2 = 0^\circ$ (at infinity).
    *   $\alpha_1$: Consider the triangle formed by the origin, the point $(-3,0,0)$ on the axis, and $P(-3,4,0)$.
    *   $\cos \alpha_1 = \frac{3}{\sqrt{3^2 + 4^2}} = \frac{3}{5}$.
*   **Direction:**
    *   Current is along $a_l=\mathbf{a}_x$ (towards origin)
    *   $\mathbf{a}_\phi =a_l \times a_p =\mathbf{a}_x \times \mathbf{a}_y = \mathbf{a}_z$.
*   **Calculating $\mathbf{H}_1$:**
   
    The text uses:
    $$ \mathbf{H}_1 = \frac{3}{4\pi(4)} \left(1 - \frac{3}{5}\right) \mathbf{a}_z $$
    $$ \mathbf{H}_1 = \frac{3}{16\pi} \left(\frac{2}{5}\right) \mathbf{a}_z = 23.87 \mathbf{a}_z \text{ mA/m} $$

#### **3. Total Field**
$$ \mathbf{H} = \mathbf{H}_1 + \mathbf{H}_2 = 38.2\mathbf{a}_x + 28.65\mathbf{a}_y + 23.87\mathbf{a}_z \text{ mA/m} $$


---

### **Practice Exercise 7.2: The positive $y$-axis (semi-infinite line with respect to the origin) carries a filamentary current of $2 \text{ A}$ in the $-\mathbf{a}_y$ direction. Find $\mathbf{H}$ at: (a) $A(2, 3, 0)$, (b) $B(3, 12, -4)$**


**Configuration:** Current flows from $+\infty$ down to the origin $(0,0,0)$ along the $y$-axis. Magnitude $I = 2 \text{ A}$.

#### **Part (a): Point $A(2, 3, 0)$**
*   **Radial Distance ($\rho$):** The perpendicular distance from the $y$-axis to point $(2,3,0)$ is the $x$-distance.
    $$ \rho = 2 \text{ m} $$
*   **Geometry Factor (Angles):**
    *   The wire exists for $y \in [0, \infty)$.
    *   Angle to $\infty$: $0^\circ \rightarrow \cos = 1$.
    *   Angle to Origin ($0,0,0$): The vertical distance is $3$, horizontal distance is $2$.
        $$ \cos \alpha = \frac{3}{\sqrt{2^2 + 3^2}} = \frac{3}{\sqrt{13}} $$
    *   Since the point ($y=3$) is between the start ($y=\infty$) and end ($y=0$) of the wire, the ==angles add up==.
    *   Magnitude Factor: $\left(1 + \frac{3}{\sqrt{13}}\right)$.
*   **Direction:**
    *   Current $\mathbf{I}$ is in $-\mathbf{a}_y$.
    *   Radial vector $\mathbf{a}_\rho$ is in $+\mathbf{a}_x$.
    *   Cross product: $(-\mathbf{a}_y) \times (\mathbf{a}_x) = \mathbf{a}_z$.
*   **Calculation:**
    $$ \mathbf{H} = \frac{I}{4\pi\rho} \left( 1 + \frac{3}{\sqrt{13}} \right) \mathbf{a}_z $$
    $$ \mathbf{H} = \frac{2}{4\pi(2)} \left( 1 + 0.832 \right) \mathbf{a}_z = \frac{1}{4\pi} (1.832) \mathbf{a}_z $$
    $$ \mathbf{H} \approx 0.1458 \mathbf{a}_z \text{ A/m} = \mathbf{145.8 \mathbf{a}_z \text{ mA/m}} $$

#### **Part (b): Point $B(3, 12, -4)$**
*   **Radial Distance ($\rho$):** Distance from $y$-axis. Point has $x=3, z=-4$.
    $$ \rho = \sqrt{3^2 + (-4)^2} = 5 \text{ m} $$
*   **Geometry Factor (Angles):**
    *   Wire: $y \in [0, \infty)$. Point is at $y=12$.
    *   Cos Angle to $\infty \rightarrow 1$.
    *   Angle to Origin: Y distance is $12$, and ($\rho$) is $5$.
    *   $\cos \alpha = \frac{12}{\sqrt{12^2 + 5^2}} = \frac{12}{13}$.
    *   Factor: $\left(1 + \frac{12}{13}\right)$. add up bcz point inside
*   **Direction:**
    *   Current: $-\mathbf{a}_y$.
    *   Vector from axis to point: $3\mathbf{a}_x - 4\mathbf{a}_z$.
    *   $\mathbf{a}_\rho = \frac{3\mathbf{a}_x - 4\mathbf{a}_z}{5}$.
    *   $\mathbf{a}_\phi = (-\mathbf{a}_y) \times \left( \frac{3\mathbf{a}_x - 4\mathbf{a}_z}{5} \right)$.
    *   $\mathbf{a}_\phi = \frac{1}{5} [ (- \mathbf{a}_y \times 3\mathbf{a}_x) - (-\mathbf{a}_y \times 4\mathbf{a}_z) ]$.
    *   $\mathbf{a}_\phi =\frac{1}{5} [ 3(\mathbf{a}_z) + 4(\mathbf{a}_x) ]  = 0.8\mathbf{a}_x + 0.6\mathbf{a}_z$.
*   **Calculation:**
    $$ H_{mag} = \frac{2}{4\pi(5)} \left( 1 + \frac{12}{13} \right) = \frac{1}{10\pi} \left( \frac{25}{13} \right) \approx 0.0612 \text{ A/m} $$
    $$ \mathbf{H} = 61.2 \text{ mA/m} \times (0.8\mathbf{a}_x + 0.6\mathbf{a}_z) $$
    $$ \mathbf{H} = \mathbf{48.97 \mathbf{a}_x + 36.73 \mathbf{a}_z \text{ mA/m}} $$


---

### **Example 7.3: A circular loop located on $x^2 + y^2 = 9, z=0$ carries a direct current of $10 \text{ A}$ along $\mathbf{a}_\phi$. Determine $\mathbf{H}$ at $(0, 0, 4)$ and $(0, 0, -4)$.**

![[Pasted image 20260119193619.png]]
This example derives the general formula for a circular loop and then applies it.

#### **1. Derivation of the Formula**
Using the Biot-Savart Law:
$$ d\mathbf{H} = \frac{I d\mathbf{l} \times \mathbf{R}}{4\pi |R|^3} $$

*   **Source ($dl$):** Located on the ring at radius $\rho$.
    $$ d\mathbf{l} = \rho \, d\phi \, \mathbf{a}_\phi $$
*   **Vector $\mathbf{R}$:** From source point $(\rho, \phi, 0)$ to observation point $(0, 0, h)$.
- **Target Point:** $(0, 0, h)$ (On the $z$-axis).
- **Source Point:** $(x, y, 0)$ (On the loop).
1. Cartesian Difference: $$\mathbf{R} = (0-x)\mathbf{a}_x + (0-y)\mathbf{a}_y + (h-0)\mathbf{a}_z = -x\mathbf{a}_x - y\mathbf{a}_y + h\mathbf{a}_z$$
    
2. **Cylindrical Conversion:**
    
    - Radial distance: $\rho = \sqrt{x^2 + y^2}$
        
    - Directional mapping: $-(x\mathbf{a}_x + y\mathbf{a}_y) = -\rho \mathbf{a}_\rho$
    
$$\mathbf{R} = -\rho \mathbf{a}_\rho + h \mathbf{a}_z$$
*   **Cross Product ($d\mathbf{l} \times \mathbf{R}$):**
    $$ (\rho \, d\phi \, \mathbf{a}_\phi) \times (-\rho \mathbf{a}_\rho + h \mathbf{a}_z) $$
$$ = -\rho^2 \, d\phi (\mathbf{a}_\phi \times \mathbf{a}_\rho) + \rho h \, d\phi (\mathbf{a}_\phi \times \mathbf{a}_z) $$
$$ = \rho h \, d\phi \, \mathbf{a}_\rho + \rho^2 \, d\phi \, \mathbf{a}_z $$
    *(Note: $\mathbf{a}_\phi \times \mathbf{a}_\rho = -\mathbf{a}_z$. The text simplifies the vector components differently, arguing by symmetry).
*   **Symmetry Argument:**
    The radial components ($\mathbf{a}_\rho$) cancel out when integrated around the whole circle (0 to $2\pi$). Only the $\mathbf{a}_z$ component survives.
*   **Integration:**
    $$ \mathbf{H} = \int_0^{2\pi} \frac{I \rho^2 d\phi \mathbf{a}_z}{4\pi (\rho^2 + h^2)^{3/2}} $$
    $$ \mathbf{H} = \frac{I \rho^2 (2\pi) \mathbf{a}_z}{4\pi (\rho^2 + h^2)^{3/2}} $$
    **Final Formula:**
    $$ \mathbf{H} = \frac{I \rho^2}{2(\rho^2 + h^2)^{3/2}} \mathbf{a}_z $$

#### **2. Application to Problem**
*   **Given:**
    *   Current $I = 10 \text{ A}$.
    *   Loop Radius $\rho = \sqrt{9} = 3 \text{ m}$.
    *   Height $h = 4 \text{ m}$.
*   **At $(0, 0, 4)$:**
    $$ \mathbf{H} = \frac{10 (3^2)}{2(3^2 + 4^2)^{3/2}} \mathbf{a}_z $$
    $$ \mathbf{H} = \frac{90}{2(9 + 16)^{3/2}} \mathbf{a}_z = \frac{45}{(25)^{3/2}} \mathbf{a}_z = \frac{45}{125} \mathbf{a}_z $$
    $$ \mathbf{H} = \mathbf{0.36 \mathbf{a}_z \text{ A/m}} $$
*   **At $(0, 0, -4)$:**
    Due to symmetry, the field direction and magnitude on the axis depend on the square of $h$   ($h^2$). Therefore, the result is identical.
    $$ \mathbf{H} = \mathbf{0.36 \mathbf{a}_z \text{ A/m}} $$

---

### **Practice Exercise 7.3: A thin ring of radius $5 \text{ cm}$ is placed on plane $z = 1 \text{ cm}$ so that its center is at $(0, 0, 1 \text{ cm})$. If the ring carries $50 \text{ mA}$ along $\mathbf{a}_\phi$, find $\mathbf{H}$ at: (a) $(0, 0, -1 \text{ cm})$, (b) $(0, 0, 10 \text{ cm})$**


This problem utilizes the formula derived in Example 7.3, but we must carefully determine $h$, which is the distance from the center of the ring to the observation point.

**Constants:**
*   Radius $\rho = 5 \text{ cm} = 0.05 \text{ m}$.
*   Current $I = 50 \text{ mA} = 0.05 \text{ A}$.
*   Center of ring $z_{center} = 1 \text{ cm} = 0.01 \text{ m}$.

**Formula:**
$$ \mathbf{H} = \frac{I \rho^2}{2(\rho^2 + h^2)^{3/2}} \mathbf{a}_z $$

#### **Part (a): Point $(0, 0, -1 \text{ cm})$**
*   **Calculate $h$:**
    The point is at $z = -1 \text{ cm}$. The ring is at $z = 1 \text{ cm}$.
    $$ h = |1 - (-1)| = 2 \text{ cm} = 0.02 \text{ m} $$
*   **Substitute Values:**
    *   Numerator: $I \rho^2 = 0.05 \times (0.05)^2 = 0.05 \times 0.0025 = 1.25 \times 10^{-4}$.
    *   Denominator term $(\rho^2 + h^2)$: $(0.05)^2 + (0.02)^2 = 0.0025 + 0.0004 = 0.0029$.
    *   Denominator: $2 \times (0.0029)^{1.5}$.
*   **Calculation:**
    $$ \mathbf{H} = \frac{1.25 \times 10^{-4}}{2 \times (0.0029)^{1.5}} \mathbf{a}_z $$
    $$ (0.0029)^{1.5} \approx 1.56 \times 10^{-4} $$
    $$ \mathbf{H} \approx \frac{1.25 \times 10^{-4}}{3.12 \times 10^{-4}} \mathbf{a}_z \approx 0.4 \mathbf{a}_z \text{ A/m} $$
*   **Convert to mA/m:**
    $$ \mathbf{H} = \mathbf{400 \mathbf{a}_z \text{ mA/m}} $$

#### **Part (b): Point $(0, 0, 10 \text{ cm})$**
*   **Calculate $h$:**
    The point is at $z = 10 \text{ cm}$. The ring is at $z = 1 \text{ cm}$.
    $$ h = |10 - 1| = 9 \text{ cm} = 0.09 \text{ m} $$
*   **Substitute Values:**
    *   Numerator: $1.25 \times 10^{-4}$ (same as above).
    *   Denominator term $(\rho^2 + h^2)$: $(0.05)^2 + (0.09)^2 = 0.0025 + 0.0081 = 0.0106$.
    *   Denominator: $2 \times (0.0106)^{1.5}$.
*   **Calculation:**
    $$ (0.0106)^{1.5} \approx 0.00109 $$
    $$ \mathbf{H} = \frac{1.25 \times 10^{-4}}{2 \times 0.00109} \mathbf{a}_z = \frac{1.25 \times 10^{-4}}{0.00218} \mathbf{a}_z $$
    $$ \mathbf{H} \approx 0.0573 \mathbf{a}_z \text{ A/m} $$
*   **Convert to mA/m:**
    $$ \mathbf{H} = \mathbf{57.3 \mathbf{a}_z \text{ mA/m}} $$  
Here is the comprehensive explanation of the examples presented in the text, covering the calculation of Magnetic Flux Density ($\mathbf{B}$) using both Magnetic Vector Potential ($\mathbf{A}$) and the Biot-Savart Law.

---

### **Example 6-4**

### **Question**
**A direct current $I$ flows in a straight wire of length $2L$. Find the magnetic flux density $\mathbf{B}$ at a point located at a distance $r$ from the wire in the bisecting plane:**
**(a) by determining the vector magnetic potential $\mathbf{A}$ first, and**
**(b) by applying the Biot-Savart law.**

**Context:**
*   The wire is aligned with the $z$-axis.
*   The wire extends from $z = -L$ to $z = +L$.
*   The observation point $P$ is at cylindrical coordinates $(r, 0, 0)$.
*   Current flows in the $+\mathbf{a}_z$ direction.

---

### **Solution Part (a): Using Vector Magnetic Potential $\mathbf{A}$**

This method involves finding the potential field $\mathbf{A}$ first, then performing a curl operation ($\nabla \times \mathbf{A}$) to find the magnetic field $\mathbf{B}$.

**1. Define the Differential Element:**
*   The current element is $d\mathbf{l}' = dz' \mathbf{a}_z$.
*   The distance $R$ from a source element at $z'$ to the point $P$ at $r$ is the hypotenuse of the triangle formed by $r$ and $z'$:
    $$ R = \sqrt{z'^2 + r^2} $$

**2. Setup the Integral for $\mathbf{A}$:**
The general formula for vector potential is:
$$ \mathbf{A} = \frac{\mu_0 I}{4\pi} \oint \frac{d\mathbf{l}'}{R} $$
Substituting our specific geometry:
$$ \mathbf{A} = \mathbf{a}_z \frac{\mu_0 I}{4\pi} \int_{-L}^{L} \frac{dz'}{\sqrt{z'^2 + r^2}} $$

**3. Evaluate the Integral:**
Using the standard integral form $\int \frac{dx}{\sqrt{x^2 + a^2}} = \ln(x + \sqrt{x^2 + a^2})$:
$$ \mathbf{A} = \mathbf{a}_z \frac{\mu_0 I}{4\pi} \left[ \ln(z' + \sqrt{z'^2 + r^2}) \right]_{-L}^{L} $$
Applying the limits ($L$ and $-L$) and simplifying using logarithm rules ($\ln A - \ln B = \ln(A/B)$):
$$ \mathbf{A} = \mathbf{a}_z \frac{\mu_0 I}{4\pi} \ln \left[ \frac{\sqrt{L^2 + r^2} + L}{\sqrt{L^2 + r^2} - L} \right] $$

**4. Calculate $\mathbf{B}$ using Curl ($\nabla \times \mathbf{A}$):**
In cylindrical coordinates, the curl of $\mathbf{A}$ is:
$$ \mathbf{B} = \nabla \times \mathbf{A} = \left( \frac{1}{r}\frac{\partial A_z}{\partial \phi} - \frac{\partial A_\phi}{\partial z} \right)\mathbf{a}_r + \left( \frac{\partial A_r}{\partial z} - \frac{\partial A_z}{\partial r} \right)\mathbf{a}_\phi + \frac{1}{r}\left( \frac{\partial (r A_\phi)}{\partial r} - \frac{\partial A_r}{\partial \phi} \right)\mathbf{a}_z $$

*   Since $\mathbf{A}$ only has a $z$-component ($A_z$), and due to cylindrical symmetry ($A_z$ does not change with $\phi$), the only surviving term is:
    $$ \mathbf{B} = - \frac{\partial A_z}{\partial r} \mathbf{a}_\phi $$

**5. Perform the Differentiation:**
Differentiating the logarithmic expression with respect to $r$ yields:
$$ \frac{\partial A_z}{\partial r} = \frac{\mu_0 I}{4\pi} \frac{\partial}{\partial r} \ln \left( \frac{\sqrt{L^2 + r^2} + L}{\sqrt{L^2 + r^2} - L} \right) $$
After performing the derivative algebra (chain rule):
$$ \mathbf{B} = \frac{\mu_0 I L}{2\pi r \sqrt{L^2 + r^2}} \mathbf{a}_\phi \quad \text{(Eq. 6-35)} $$

**Limiting Case (Infinite Wire):**
If the wire is infinitely long ($L \gg r$), then $\sqrt{L^2 + r^2} \approx L$. The equation simplifies to the standard Biot-Savart result for an infinite line:
$$ \mathbf{B} = \frac{\mu_0 I}{2\pi r} \mathbf{a}_\phi $$

---

### **Solution Part (b): Using Biot-Savart Law**

This method calculates $\mathbf{B}$ directly by integrating the differential contributions $d\mathbf{B}$.

**1. Define Vectors:**
*   Source vector (position of current element): $\mathbf{r}' = z' \mathbf{a}_z$
*   Field vector (position of point $P$): $\mathbf{r}_p = r \mathbf{a}_r$
*   Distance vector $\mathbf{R} = \mathbf{r}_p - \mathbf{r}' = r \mathbf{a}_r - z' \mathbf{a}_z$
*   Magnitude $R = \sqrt{r^2 + z'^2}$

**2. The Cross Product ($d\mathbf{l}' \times \mathbf{R}$):**
$$ d\mathbf{l}' = dz' \mathbf{a}_z $$
$$ d\mathbf{l}' \times \mathbf{R} = (dz' \mathbf{a}_z) \times (r \mathbf{a}_r - z' \mathbf{a}_z) $$
Using cross product rules ($\mathbf{a}_z \times \mathbf{a}_r = \mathbf{a}_\phi$ and $\mathbf{a}_z \times \mathbf{a}_z = 0$):
$$ d\mathbf{l}' \times \mathbf{R} = r \, dz' \, \mathbf{a}_\phi $$

**3. Setup the Integral:**
$$ \mathbf{B} = \int_{-L}^{L} \frac{\mu_0 I (r \, dz')}{4\pi (z'^2 + r^2)^{3/2}} \mathbf{a}_\phi $$

**4. Solve the Integral:**
Using standard integral tables or trigonometric substitution ($z' = r \tan \theta$):
$$ \int \frac{dz'}{(z'^2 + r^2)^{3/2}} = \frac{z'}{r^2 \sqrt{z'^2 + r^2}} $$
Evaluating from $-L$ to $L$:
$$ \mathbf{B} = \frac{\mu_0 I r}{4\pi} \left[ \frac{z'}{r^2 \sqrt{z'^2 + r^2}} \right]_{-L}^{L} \mathbf{a}_\phi $$
$$ \mathbf{B} = \frac{\mu_0 I r}{4\pi r^2} \left( \frac{L}{\sqrt{L^2 + r^2}} - \frac{-L}{\sqrt{L^2 + r^2}} \right) \mathbf{a}_\phi $$
$$ \mathbf{B} = \frac{\mu_0 I L}{2\pi r \sqrt{L^2 + r^2}} \mathbf{a}_\phi $$

*This result matches exactly with the result found in Part (a).*

---

### **Example 6-5**

### **Question**
**Find the magnetic flux density at the center of a square loop, with side $w$ carrying a direct current $I$.**

**Context:**
*   A square loop lies in the $xy$-plane.
*   Side length is $w$.
*   We need the field at the geometric center.

### **Solution**

**1. Principle of Superposition:**
The total magnetic field is the sum of the fields produced by the four individual sides of the square.
$$ \mathbf{B}_{total} = \mathbf{B}_{side1} + \mathbf{B}_{side2} + \mathbf{B}_{side3} + \mathbf{B}_{side4} $$
By symmetry, the magnitude of the field from each side is identical, and they all point in the same direction (along the $z$-axis, assuming counter-clockwise current). Thus:
$$ \mathbf{B}_{total} = 4 \times \mathbf{B}_{one\_side} $$

**2. Adapt Formula from Example 6-4:**
We treat one side of the square as a finite straight wire of length $2L = w$.
*   Length of wire ($2L$): $w \implies L = w/2$.
*   Distance from wire to center ($r$): $w/2$.

Substitute these into Eq. 6-35 ($\mathbf{B} = \frac{\mu_0 I L}{2\pi r \sqrt{L^2 + r^2}}$):

$$ B_{one\_side} = \frac{\mu_0 I (w/2)}{2\pi (w/2) \sqrt{(w/2)^2 + (w/2)^2}} $$

**3. Simplify:**
$$ B_{one\_side} = \frac{\mu_0 I}{2\pi \sqrt{2(w/2)^2}} = \frac{\mu_0 I}{2\pi (w/2)\sqrt{2}} = \frac{\mu_0 I}{\pi w \sqrt{2}} $$
Rationalizing the denominator (multiplying numerator and denominator by $\sqrt{2}$):
$$ B_{one\_side} = \frac{\sqrt{2}\mu_0 I}{2\pi w} $$

**4. Calculate Total Field:**
Multiply by 4 sides:
$$ \mathbf{B}_{total} = 4 \times \left( \frac{\sqrt{2}\mu_0 I}{2\pi w} \right) \mathbf{a}_z $$
$$ \mathbf{B}_{total} = \frac{2\sqrt{2}\mu_0 I}{\pi w} \mathbf{a}_z $$

---

### **Example 6-6**

### **Question**
**Find the magnetic flux density at a point on the axis of a circular loop of radius $b$ that carries a direct current $I$.**

**Context:**
*   Loop is in the $xy$-plane, centered at the origin.
*   Radius is $b$.
*   Current $I$ flows in the $\mathbf{a}_\phi$ direction.
*   Observation point $P$ is at $(0, 0, z)$.

### **Solution**

We apply the Biot-Savart Law directly.

**1. Differential Element ($d\mathbf{l}'$):**
A small segment of the loop at radius $b$:
$$ d\mathbf{l}' = b \, d\phi' \, \mathbf{a}_\phi $$

**2. Distance Vector ($\mathbf{R}$):**
*   From source $(b, \phi', 0)$ to point $(0, 0, z)$:
*   $\mathbf{R} = z \mathbf{a}_z - b \mathbf{a}_\rho$ (Note: $\mathbf{a}_\rho$ is the radial unit vector in the cylindrical plane).
*   Magnitude: $R = \sqrt{z^2 + b^2}$.

**3. Cross Product ($d\mathbf{l}' \times \mathbf{R}$):**
$$ d\mathbf{l}' \times \mathbf{R} = (b \, d\phi' \, \mathbf{a}_\phi) \times (z \mathbf{a}_z - b \mathbf{a}_\rho) $$
Distributing the cross product:
1.  $\mathbf{a}_\phi \times \mathbf{a}_z = \mathbf{a}_\rho$
2.  $\mathbf{a}_\phi \times \mathbf{a}_\rho = -\mathbf{a}_z$

$$ d\mathbf{l}' \times \mathbf{R} = (b z \, d\phi') \mathbf{a}_\rho + (b^2 \, d\phi') \mathbf{a}_z $$

**4. Symmetry Argument:**
*   The term with $\mathbf{a}_\rho$ represents the radial component of the field.
*   For every element on the loop at angle $\phi$, there is a diametrically opposite element at $\phi + \pi$. Their radial contributions cancel out.
*   Therefore, we only integrate the $\mathbf{a}_z$ component.

**5. Perform the Integration:**
$$ \mathbf{B} = \int_{0}^{2\pi} \frac{\mu_0 I (b^2 \, d\phi')}{4\pi (z^2 + b^2)^{3/2}} \mathbf{a}_z $$

Since $I, b, z$ are all constant with respect to $\phi'$, they move outside the integral:
$$ \mathbf{B} = \frac{\mu_0 I b^2}{4\pi (z^2 + b^2)^{3/2}} \mathbf{a}_z \int_{0}^{2\pi} d\phi' $$
$$ \mathbf{B} = \frac{\mu_0 I b^2}{4\pi (z^2 + b^2)^{3/2}} (2\pi) \mathbf{a}_z $$

**6. Final Result:**
$$ \mathbf{B} = \frac{\mu_0 I b^2}{2(z^2 + b^2)^{3/2}} \mathbf{a}_z $$

**Special Case (Center of the loop):**
If $z = 0$, the formula simplifies to:
$$ \mathbf{B} = \frac{\mu_0 I}{2b} \mathbf{a}_z $$